\documentclass[journal,12pt,twocolumn]{IEEEtran}

\usepackage{enumitem}
\usepackage{amsmath}
\usepackage{amssymb}
\usepackage{gensymb}
\usepackage{graphicx}
\usepackage{txfonts}         
\usepackage{listings}
\usepackage{lstautogobble}
\usepackage{mathtools}
\usepackage{bm}
\usepackage{hyperref}
\usepackage{polynom}
\usepackage{capt-of}
\usepackage{siunitx}
\newcommand{\solution}{\noindent \textbf{Solution: }}
\providecommand{\pr}[1]{\ensuremath{\Pr\left(#1\right)}}
\providecommand{\brak}[1]{\ensuremath{\left(#1\right)}}
\providecommand{\cbrak}[1]{\ensuremath{\left\{#1\right\}}}
\providecommand{\sbrak}[1]{\ensuremath{\left[#1\right]}}
\providecommand{\mean}[1]{E\left[ #1 \right]}
\providecommand{\var}[1]{\mathrm{Var}\left[ #1 \right]}
\providecommand{\der}[1]{\mathrm{d} #1}
\providecommand{\gauss}[2]{\mathcal{N}\ensuremath{\left(#1,#2\right)}}
\providecommand{\mbf}{\mathbf}
\providecommand{\abs}[1]{\left\vert#1\right\vert}
\providecommand{\norm}[1]{\left\lVert#1\right\rVert}
\providecommand{\z}[1]{{\mathcal{Z}}\{#1\}}
\providecommand{\ztrans}{\overset{\mathcal{Z}}{ \rightleftharpoons}}

\providecommand{\parder}[2]{\frac{\partial}{\partial #2} \brak{#1}}

\let\StandardTheFigure\thefigure
\let\vec\mathbf

\numberwithin{equation}{section}
\renewcommand{\thefigure}{\theenumi}
\renewcommand\thesection{\arabic{section}}

\newcommand{\myvec}[1]{\ensuremath{\begin{pmatrix}#1\end{pmatrix}}}
\newcommand{\mydet}[1]{\ensuremath{\begin{vmatrix}#1\end{vmatrix}}}
\newcommand{\define}{\stackrel{\triangle}{=}}

\DeclareMathOperator*{\argmin}{arg\,min}
\DeclareMathOperator*{\argmax}{arg\,max}

\makeatletter
\def\pld@CF@loop#1+{%
    \ifx\relax#1\else
        \begingroup
          \pld@AccuSetX11%
          \def\pld@frac{{}{}}\let\pld@symbols\@empty\let\pld@vars\@empty
          \pld@false
          #1%
          \let\pld@temp\@empty
          \pld@AccuIfOne{}{\pld@AccuGet\pld@temp
                            \edef\pld@temp{\noexpand\pld@R\pld@temp}}%
           \pld@if \pld@Extend\pld@temp{\expandafter\pld@F\pld@frac}\fi
           \expandafter\pld@CF@loop@\pld@symbols\relax\@empty
           \expandafter\pld@CF@loop@\pld@vars\relax\@empty
           \ifx\@empty\pld@temp
               \def\pld@temp{\pld@R11}%
           \fi
          \global\let\@gtempa\pld@temp
        \endgroup
        \ifx\@empty\@gtempa\else
            \pld@ExtendPoly\pld@tempoly\@gtempa
        \fi
        \expandafter\pld@CF@loop
    \fi}
\def\pld@CMAddToTempoly{%
    \pld@AccuGet\pld@temp\edef\pld@temp{\noexpand\pld@R\pld@temp}%
    \pld@CondenseMonomials\pld@false\pld@symbols
    \ifx\pld@symbols\@empty \else
        \pld@ExtendPoly\pld@temp\pld@symbols
    \fi
    \ifx\pld@temp\@empty \else
        \pld@if
            \expandafter\pld@IfSum\expandafter{\pld@temp}%
                {\expandafter\def\expandafter\pld@temp\expandafter
                    {\expandafter\pld@F\expandafter{\pld@temp}{}}}%
                {}%
        \fi
        \pld@ExtendPoly\pld@tempoly\pld@temp
        \pld@Extend\pld@tempoly{\pld@monom}%
    \fi}
\makeatother

\lstset {
	frame=single, 
	breaklines=true,
	columns=fullflexible,
	autogobble=true
}             
   


\begin{document}
                             
\title{ Digital Signal Processing \\ \Large EE3900: Linear Systems and Signal Processing \\ \large Indian Institute of Technology Hyderabad}
\author{Aakash Kamuju \\ \normalsize AI21BTECH11001 \\ \vspace*{20pt} \normalsize 1 Aug 2022}   
 \maketitle 
 \tableofcontents

%\renewcommand{\thefigure}{\thesection.\theenumi}
%\renewcommand{\thetable}{\thesection.\theenumi}

\renewcommand{\thefigure}{\theenumi}
\renewcommand{\thetable}{\theenumi}

%\renewcommand{\theequation}{\thesection}


\bigskip

\begin{abstract}
This manual provides a simple introduction to digital signal processing.
\end{abstract}
\section{Software Installation}
Run the following commands
\begin{lstlisting}
sudo apt-get update
sudo apt-get install libffi-dev libsndfile1 python3-scipy  python3-numpy python3-matplotlib 
sudo pip install cffi pysoundfile 
\end{lstlisting}
\section{Digital Filter}
\begin{enumerate}[label=\thesection.\arabic*
,ref=\thesection.\theenumi]
\item
\label{prob:input}
Download the sound file from  
\begin{lstlisting}
wget https://github.com/kamujuaakash/EE3900/blob/main/codes/Sound_Noise.wav
\end{lstlisting}
%\href{http://tlc.iith.ac.in/img/sound/Sound_Noise.wav}{\url{http://tlc.iith.ac.in/img/sound/Sound_Noise.wav}}  
%in the link given below.
%\linebreak
\item
\label{prob:spectrogram}
You will find a spectrogram at \href{https://academo.org/demos/spectrum-analyzer}{\url{https://academo.org/demos/spectrum-analyzer}}. 
%\end{problem}
%%
%
%%\onecolumn
%%\input{./figs/fir}
%\begin{problem}
Upload the sound file that you downloaded in Problem \ref{prob:input} in the spectrogram  and play.  Observe the spectrogram. What do you find?
\\
%
\solution There are a lot of yellow lines between 440 Hz to 5.1 KHz.  These represent the synthesizer key tones. Also, the key strokes
are audible along with background noise.
% By observing spectrogram, it clearly shows that tonal frequency is under 4kHz. And above 4kHz only noise is present.
\item
\label{prob:output}
Write the python code for removal of out of band noise and execute the code.
\\
\solution
\lstinputlisting{./codes/Cancel_noise.py}
%\begin{figure}[h]
%\centering
%\includegraphics[width=\columnwidth]{enc_block_diag.png}
%\caption{}
%\label{fig:convolution encoder}
%\end{figure}
%\input{block_enc}
\item
The output of the python script in Problem \ref{prob:output} is the audio file Sound\_With\_ReducedNoise.wav. Play the file in the spectrogram in Problem \ref{prob:spectrogram}. What do you observe?
\\
\solution The key strokes as well as background noise is subdued in the audio.  Also,  the signal is blank for frequencies above 5.1 kHz.

\end{enumerate}
\section{Difference Equation}
\begin{enumerate}[label=\thesection.\arabic*,ref=\thesection.\theenumi]
\item Let
\begin{equation}
x(n) = \cbrak{\underset{\uparrow}{1},2,3,4,2,1}
\end{equation}
Sketch $x(n)$.
\\
\solution The following code yields Fig. \ref{fig:3.1}
\begin{lstlisting}
wget https://github.com/kamujuaakash/EE3900/blob/main/codes/3.1.py
\end{lstlisting}
\begin{figure}[!ht]
\begin{center}
\includegraphics[width=\columnwidth]{./figs/3.1}
\end{center}
\captionof{figure}{}
\label{fig:3.1}	
\end{figure}
\item Let
\begin{multline}
\label{eq:iir_filter}
y(n) + \frac{1}{2}y(n-1) = x(n) + x(n-2), 
\\
 y(n) = 0, n < 0
\end{multline}
Sketch $y(n)$.
\\
\solution The following code yields Fig. \ref{fig:xnyn}.
\begin{lstlisting}
wget https://github.com/kamujuaakash/EE3900/blob/main/codes/xnyn.py
\end{lstlisting}
\begin{figure}[!ht]
\begin{center}
\includegraphics[width=\columnwidth]{./figs/xnyn}
\end{center}
\captionof{figure}{}
\label{fig:xnyn}	
\end{figure}

\end{enumerate}
\section{$Z$-transform}
\begin{enumerate}[label=\thesection.\arabic*]
\item The $Z$-transform of $x(n)$ is defined as
%
\begin{equation}
\label{eq:z_trans}
X(z)={\mathcal {Z}}\{x(n)\}=\sum _{n=-\infty }^{\infty }x(n)z^{-n}
\end{equation}
%
Show that
\begin{equation}
\label{eq:shift1}
{\mathcal {Z}}\{x(n-1)\} = z^{-1}X(z)
\end{equation}
and find
\begin{equation}
	{\mathcal {Z}}\{x(n-k)\} 
\end{equation}
\solution From \eqref{eq:z_trans},
\begin{align}
{\mathcal {Z}}\{x(n-k)\} &=\sum _{n=-\infty }^{\infty }x(n-1)z^{-n}
\\
&=\sum _{n=-\infty }^{\infty }x(n)z^{-n-1} = z^{-1}\sum _{n=-\infty }^{\infty }x(n)z^{-n}
\end{align}
resulting in \eqref{eq:shift1}. Similarly, it can be shown that
%
\begin{equation}
\label{eq:z_trans_shift}
	{\mathcal {Z}}\{x(n-k)\} = z^{-k}X(z)
\end{equation}
\item Obtain $X(z)$ for x(n) define in problem 3.1.
\solution From \eqref{eq:z_trans},
\begin{align}
X(z)&={\mathcal{Z}}\{x(n)\}=\sum_{n=-\infty}^{\infty}x(n)z^{-n}\\
\label{eq:genf}
&=\sum_{n=0}^{\infty}x(n)z^{-n}\\
&=1\cdot z^{-1}+2\cdot z^{-2}+3\cdot z^{-3}+4\cdot z^{-4}+2\cdot z^{-5}+1\cdot z^{-6}\\
&=\frac{z^5+2z^4+3z^3++4z^2+2z+1}{z^6}
\end{align}
\item Find
%
\begin{equation}
H(z) = \frac{Y(z)}{X(z)}
\end{equation}
%
from  \eqref{eq:iir_filter} assuming that the $Z$-transform is a linear operation.
\\
\solution  Applying \eqref{eq:z_trans_shift} in \eqref{eq:iir_filter},
\begin{align}
Y(z) + \frac{1}{2}z^{-1}Y(z) &= X(z)+z^{-2}X(z)
\\
\implies H\brak{z} = \frac{Y(z)}{X(z)} &= \frac{1 + z^{-2}}{1 + \frac{1}{2}z^{-1}}
\label{eq:freq_resp}
\end{align}
%
\item Find the Z transform of 
\begin{equation}
\delta(n)
=
\begin{cases}
1 & n = 0
\\
0 & \text{otherwise}
\end{cases}
\end{equation}
and show that the $Z$-transform of
\begin{equation}
\label{eq:unit_step}
u(n)
=
\begin{cases}
1 & n \ge 0
\\
0 & \text{otherwise}
\end{cases}
\end{equation}
is
\begin{equation}
U(z) = \frac{1}{1-z^{-1}}, \quad \abs{z} > 1
\end{equation}
\solution It is easy to show that
\begin{equation}
\delta(n) \ztrans 1
\end{equation}
and from \eqref{eq:unit_step},
\begin{align}
U(z) &= \sum _{n= 0}^{\infty}z^{-n}
\\
&=\frac{1}{1-z^{-1}}, \quad \abs{z} > 1
\end{align}
using the fomula for the sum of an infinite geometric progression.
%
\item Show that 
\begin{equation}
\label{eq:anun}
a^nu(n) \ztrans \frac{1}{1-az^{-1}} \quad \abs{z} > \abs{a}
\end{equation}
\solution From \eqref{eq:z_trans},
\begin{equation}
{\mathcal {Z}}\{a^nu(n)\} = \sum _{n= -\infty}^{\infty}u(n)\brak{\frac{a}{z}}^{-n}
\end{equation}
From \eqref{eq:unit_step},
\begin{align}
{\mathcal {Z}}\{a^nu(n)\} &= \sum _{n= 0}^{\infty}\brak{\frac{a}{z}}^{-n}\\
&= \frac{1}{1-\frac{a}{z}}\\
&= \frac{1}{1-az^{-1}} \quad \abs{z} > \abs{a}
\end{align}
using the formula for the sum of an infinite geometric progression.

%
\item 
Let
\begin{equation}
H\brak{e^{\j \omega}} = H\brak{z = e^{\j \omega}}.
\end{equation}
Plot $\abs{H\brak{e^{\j \omega}}}$. Is it periodic? If so,find the period. $H(e^{\j \omega})$ is
known as the {\em Discret Time Fourier Transform} (DTFT) of $x(n)$.
\\
\solution 
\begin{align}
H\brak{e^{\j \omega}} &= H\brak{z = e^{\j \omega}}\\
&= \frac{1 + e^{-2 \j \omega}}{1 + \frac{1}{2} e^{-\j \omega}}\\
&= \frac{2\brak{1 + e^{-2 \j \omega}}}{2 + e^{-\j \omega}}\\
&= \frac{2\brak{1 + \cos{2 \omega}-\j \sin{2\omega}}}{2 + \cos{\omega}-\j \sin{ \omega}}\\
&= \frac{2\abs{\brak{2\cos^2 \omega-\j \sin{2\omega}}}}{\abs{2 + \cos{\omega}-\j \sin{ \omega}}}\\
&= \frac{2\sqrt{4\cos^4 \omega+4\sin^2 \omega \cos^2 \omega}}{\sqrt{\brak{2 + \cos \omega}^2+ \sin^2 \omega }}\\
&=\frac{4\cos\omega}{\sqrt{5 + 4\cos \omega}}\\
\abs{H\brak{e^{\j \omega}} }&=\frac{\abs{4\cos\omega}}{\sqrt{5 + 4\cos \omega}}
\end{align}
Since $\abs{H(e^{j\omega})}$ is function of cosine we can say it is periodic.And from the plot \ref{fig:dtft} we can say that it is symmetric about $\omega = 0\brak{\text{even function}}$ and it is periodic with period $2\pi$.You can find the same from the theoritical expression $\abs{H\brak{e^{j \omega}}}$, 
       \begin{align}
         H(e^{\j \omega}) &= H(e^{j(-\omega)})\brak{\text{cos is an even function}}
       \end{align}
    And to find period, the period of $\abs{\cos(\omega)}$ is $\pi$ and the period of $\sqrt{5 + 4\cos\brak{\omega}}$ is $2\pi$. So the period of division of both will be $2\pi$.
     This gives us the period of $\abs{H(e^{j\omega})}$ as $2\pi$
 The following code plots Fig. \ref{fig:dtft}.
\begin{lstlisting}
wget https://github.com/kamujuaakash/EE3900/blob/main/codes/hn.py
\end{lstlisting}
\begin{figure}[!ht]
\centering
\includegraphics[width=\columnwidth]{./figs/dtft}
\caption{$\abs{H\brak{e^{\j\omega}}}$}
\label{fig:dtft}
\end{figure}


\item Express $h(n)$ in terms of $H\brak{e^{\j\omega}}$	
	
	\solution 
\begin{align}
\int_{-\pi}^{\pi} H(e^{\j\omega}) e^{\j\omega n} d\omega\\
= \int_{-\pi}^{\pi} \sum_{k=-\infty}^\infty h(k)  e^{-\j\omega k} e^{\j\omega n} d\omega\\
= \sum_{k=-\infty}^\infty h(k) \int_{-\pi}^{\pi} e^{\j\omega(n-k)} d\omega
\end{align}	
	Now,
	\begin{align}
		 \int_{-\pi}^{\pi} e^{\j\omega(n-k)} d\omega 
		 &= \begin{cases}
		 	\int_{-\pi}^\pi d\omega & n-k = 0 \\
		 	\left.\frac{\exp\brak{\j\omega(n-k)}}{\j(n-k)}\right|_{-\pi}^\pi & n-k \ne 0
		 \end{cases} \\		 
		 &= \begin{cases}
		 	2\pi & n-k = 0 \\
		 	0 & n-k \ne 0
		 \end{cases} \\
		 &= 2\pi \delta(n-k)
	\end{align}
	
	Thus,
	\begin{align}
		\int_{-\pi}^{\pi} H(e^{\j\omega}) e^{\j\omega n} d \omega &= 2\pi\sum_{k=-\infty}^\infty h(k) \delta(n-k) \\
		&= 2\pi h(n) * \delta(n) \\
		&= 2\pi h(n)
	\end{align}
	
	Therefore, $h(n)$ is given by the inverse DTFT (IDTFT) of $H\brak{e^{\j\omega}}$
	\begin{align}
		h(n) &= \frac{1}{2\pi} \int_{-\pi}^{\pi} H(e^{\j\omega}) e^{\j\omega n}  d \omega 
	\end{align}
\end{enumerate}

\section{Impulse Response}
\begin{enumerate}[label=\thesection.\arabic*]
\item Using long division, 
find
		\begin{align}
			h(n), \quad n < 5
		\end{align}
		for H(z) in 
		\eqref{eq:freq_resp}.\\
\solution 
	\begin{equation}
		H(z) = \frac{1 + z^{-2}}{1 + \frac12 z^{-1}}
	\end{equation}
	Substitute $z^{-1} = x$
	\polylongdiv{1+x^2}{1+\frac12 x}
	
	\begin{align}
		&\implies 1 + z^{-2} = \brak{1 + \frac12 z^{-1}}\brak{-4 + 2z^{-1}} + 5 \\
		&\implies H(z) = -4 + 2z^{-1} + \frac{5}{1 + \frac12 z^{-1}}
	\end{align}
	
	On applying the inverse $Z$-transform on both sides of the equation
	\begin{align}
		H(z) &\ztrans h(n) \\
		-4 &\ztrans -4\delta(n) \\
		2z^{-1} &\ztrans 2\delta(n - 1) \\
		\frac{5}{1 + \frac12 z^{-1}} &\ztrans 5\brak{-\frac12}^n u(n) \\
	\end{align}
	
	Therefore,
	\begin{equation}
		h(n) = -4\delta(n) + 2\delta(n - 1) + 5\brak{-\frac12}^n u(n)
	\end{equation}
\item \label{prob:impulse_resp}
Find an expression for $h(n)$ using $H(z)$, given that 
in \eqref{eq:anun}, given that
\begin{equation}
\label{eq:impulse_resp}
h(n) \ztrans H(z)
\end{equation}
and there is a one to one relationship between $h(n)$ and $H(z)$. $h(n)$ is known as the {\em impulse response} of the
system defined by \eqref{eq:iir_filter}.
\\
\solution From \eqref{eq:freq_resp},
\begin{align}
H(z) &= \frac{1}{1 + \frac{1}{2}z^{-1}} + \frac{ z^{-2}}{1 + \frac{1}{2}z^{-1}}
\\
\implies h(n) &= \brak{-\frac{1}{2}}^{n}u(n) + \brak{-\frac{1}{2}}^{n-2}u(n-2)
\end{align}
using \eqref{eq:anun} and \eqref{eq:z_trans_shift}.

\item Sketch $h(n)$. Is it bounded? Justify theoretically.
\\
\solution 

The following code plots
\begin{figure}[!ht]
\begin{center}
\includegraphics[width=\columnwidth]{./figs/hn}
\end{center}
\captionof{figure}{}
\label{fig:xnyn}	
\end{figure}
\begin{lstlisting}
wget https://github.com/kamujuaakash/EE3900/blob/main/Simulation/codes/5.3.py
\end{lstlisting}

\begin{align}
\lim_{n\to\infty}h(n)&=\lim_{n\to\infty}\brak{-\frac{1}{2}}^{n}u(n) + \lim_{n\to\infty}\brak{-\frac{1}{2}}^{n-2}u(n-2)
\end{align}
\begin{equation}
h(n)
=
\begin{cases}
5\brak{\frac{-1}{2}}^n & n \ge 2
\\
\brak{\frac{-1}{2}}^n & 0\le n < 2
\\
0 & n<0
\end{cases}
\end{equation}
Maximum value and minimum value are always bounded in this case.
$\therefore h(n)$ is bounded

 \item Is it convergent? Justify using the ratio test.
\solution
\begin{align}
h(n+1)&=\brak{-\frac{1}{2}}^{n+1}u(n+1) + \brak{-\frac{1}{2}}^{n-1}u(n-1)
\end{align}
According to ratio test, $L$ is given by $\lim_{n\to \infty}\abs{\frac{h(n+1)}{h(n)}}$, if $L < 1$ then h(n) is convergent.
\begin{align}
L&=\lim_{n\to \infty}\abs{\frac{h(n+1)}{h(n)}}\\
&=\lim_{n\to \infty}\abs{\frac{\brak{-\frac{1}{2}}^{n+1}u(n+1) + \brak{-\frac{1}{2}}^{n-1}u(n-1)}{\brak{-\frac{1}{2}}^{n}u(n) + \brak{-\frac{1}{2}}^{n-2}u(n-2)}}\\
&=\abs{\frac{-\frac{1}{2} + {-\frac{1}{2}}^{-1}}{1 + {-\frac{1}{2}}^-2}}\\
&=\abs{\frac{-\frac{1}{2}-2}{1+4}}\\
&=\abs{\frac{\frac{-5}{2}}{5}}\\
&=\frac{1}{2}
\end{align}
As $L < 1$, $h(n)$ is convergent.

\item The system with $h(n)$ is defined to be stable if
\begin{equation}
\sum_{n=-\infty}^{\infty}h(n) < \infty
\end{equation}
Is the system defined by \eqref{eq:iir_filter} stable for the impulse response in \eqref{eq:impulse_resp}?\\
\solution 
\begin{align}
\sum_{n=-\infty}^{\infty}h(n)&= \sum_{n=0}^{\infty}h(n)\\
&=\sum_{n=0}^{\infty}\brak{-\frac{1}{2}}^{n}u(n) + \sum_{n=0}^{\infty}\brak{-\frac{1}{2}}^{n-2}u(n-2)\\
&=2 \brak{ \frac{1}{1+\frac{1}{2}}}\\
&=\frac{4}{3}
\end{align}
As $\sum_{n=-\infty}^{\infty}h(n)=\frac{4}{3}$ is less than $\infty$, the system defined by (3.2) is stable for the impulse response in (5.1).
%
\item Verify the above result using a python code.
\solution The following code determines if it is convergent or not:
\begin{lstlisting}
wget https://github.com/kamujuaakash/EE3900/blob/main/Simulation/codes/5.5.py
\end{lstlisting}
%
\item 
Compute and sketch $h(n)$ using 
\begin{equation}
\label{eq:iir_filter_h}
h(n) + \frac{1}{2}h(n-1) = \delta(n) + \delta(n-2), 
\end{equation}
%
This is the definition of $h(n)$.
\\
\solution The following code plots Fig. \ref{fig:hndef}. Note that this is the same as Fig. 
\ref{fig:hn}. 
%
\begin{lstlisting}
wget https://github.com/kamujuaakash/EE3900/blob/main/Simulation/codes/5.7.py
\end{lstlisting}
Computing,\\
$h(0)=1$\\
$h(1)=-\frac{1}{2}h(0)$\\
$h(2)=-\frac{1}{2}h(1)+1$\\
Parallely, $h(n)=-\frac{1}{2}h(n-1)$

\begin{figure}[!ht]
\centering
\includegraphics[width=\columnwidth]{./figs/hndef}
\caption{$h(n)$ from the definition}
\label{fig:hndef}
\end{figure}
%
\item Compute 
%
\begin{equation}
\label{eq:convolution}
y(n) = x(n)*h(n) = \sum_{n=-\infty}^{\infty}x(k)h(n-k)
\end{equation}
%
Comment. The operation in \eqref{eq:convolution} is known as
{\em convolution}.
%
\\
\solution The following code plots Fig. \ref{fig:ynconv}. Note that this is the same as 
$y(n)$ in  Fig. 
\ref{fig:xnyn}. 
%
\begin{lstlisting}
wget https://github.com/kamujuaakash/EE3900/blob/main/Simulation/codes/5.8.py
\end{lstlisting}
\begin{figure}[!ht]
\centering
\includegraphics[width=\columnwidth]{./figs/ynconv}
\caption{$y(n)$ from the definition of convolution}
\label{fig:ynconv}
\end{figure}
\item Express the above convolution using a toeplitz matrix.
\solution
\begin{align}
\vec{y} = \vec{x} 
\circledast \vec{h}\\
& \vec{y} = \myvec{ h_1 & 0 & . & . & . & 0 \\ h_2 & h_1 & . & . & . & 0 \\ h_3 & h_2 & h_1 & . & . & 0 \\
 h_{m-1} & . & . & . & h_2 & h_1 \\ 
 h_m & h_{m-1} &. & . & . & h_2 \\ 
 . & . &. & . & . & . \\ 
 . & . & . & . & . & . \\
  0 & 0 & . & . & . & h_m } 
  \myvec{x_1 \\ x_2 \\ . \\ . \\ . \\ . \\ x_n}
\end{align}

\begin{align}
\vec{y}&=\myvec{1 & 0&0 & 0 & 0 & 0 \\ \frac{-1}{2} & 1&0&0&0&0\\\frac{5}{4}&\frac{-1}{2}&1&0&0&0\\\frac{-5}{8}&\frac{5}{4}&\frac{-1}{2}&1&0&0\\\frac{5}{16}&\frac{-5}{8}&\frac{5}{4}&\frac{-1}{2}&1&0\\ \frac{-5}{32}&\frac{5}{16}&\frac{-5}{8}&\frac{5}{4}&\frac{-1}{2}&1\\\frac{5}{64}&\frac{-5}{32}&\frac{5}{16}&\frac{-5}{8}&\frac{5}{4}&\frac{-1}{2}\\ 0&\frac{5}{64}&\frac{-5}{32}&\frac{5}{16}&\frac{-5}{8}&\frac{5}{4}\\0&0&\frac{5}{64}&\frac{-5}{32}&\frac{5}{16}&\frac{-5}{8}\\0&0&0&\frac{5}{64}&\frac{-5}{32}&\frac{5}{16}\\0&0&0&0&\frac{5}{64}&\frac{-5}{32}\\0&0&0&0&0&\frac{5}{64}}\myvec{1\\2\\3\\4\\2\\1}
&=\myvec{1.   \\     1.5\\3.25\\4.375\\2.8125   \\3.59375\\   0.203125\\
  0.9375  \\ -0.390625 \\ 0.3125   \\ 0.     \\	   0.078125}
\end{align}
And this is what we got in \eqref{eq:convolution}
\item Show that
\begin{equation}
y(n) =  \sum_{n=-\infty}^{\infty}x(n-k)h(k)
\end{equation}
\solution Substitute $k\to n-k$ then \begin{align}
y(n) &=  x(n)*h(n)\\
&=\sum_{n=-\infty}^{\infty}x(k)h(n-k)
&= \sum_{n=-\infty}^{\infty}x(n-k)h(k)
\end{align}
\end{enumerate}
%
\section{DFT and FFT}
\begin{enumerate}[label=\thesection.\arabic*]
\item
Compute
\begin{equation}
X(k) \define \sum _{n=0}^{N-1}x(n) e^{-\j2\pi kn/N}, \quad k = 0,1,\dots, N-1
\end{equation}
and $H(k)$ using $h(n)$.
\solution The following code plots Fig. \ref{fig:xkhk}. 
\begin{figure}[!ht]
\centering
\includegraphics[width=\columnwidth]{./figs/xkhk}
\caption{$X(k) ,H(k)$ from the DFT}
\label{fig:xkhk}
\end{figure}
\begin{lstlisting}
wget https://github.com/kamujuaakash/EE3900/blob/main/codes/xkhkdft.py
\end{lstlisting}
\item Compute 
\begin{equation}
Y(k) = X(k)H(k)
\end{equation}
\solution The following code plots Fig. \ref{fig:yk}. 
\begin{figure}[!ht]
\centering
\includegraphics[width=\columnwidth]{./figs/yk}
\caption{$Y(k)$ from the DFT}
\label{fig:yk}
\end{figure}
\begin{lstlisting}
wget https://github.com/kamujuaakash/EE3900/blob/main/codes/ykdft.py
\end{lstlisting}
\item Compute
\begin{equation}
 y\brak{n}={\frac {1}{N}}\sum _{k=0}^{N-1}Y\brak{k}\cdot e^{\j 2\pi kn/N},\quad n = 0,1,\dots, N-1
\end{equation}
\\
\solution The following code plots Fig. \ref{fig:ynconv}. Note that this is the same as 
$y(n)$ in  Fig. 
\ref{fig:xnyn}. 
%
\begin{lstlisting}
wget https://github.com/kamujuaakash/EE3900/blob/main/codes/yndft.py
\end{lstlisting}
\begin{figure}[!ht]
\centering
\includegraphics[width=\columnwidth]{./figs/yndft}
\caption{$y(n)$ from the DFT}
\label{fig:yndft}
\end{figure}

\item Repeat the previous exercise by computing $X(k), H(k)$ and $y(n)$ through FFT and 
IFFT.
\item Wherever possible, express all the above equations as matrix equations.
\end{enumerate}
%
\section{Exercises}

Answer the following questions by looking at the python code in Problem \ref{prob:output}.
\begin{enumerate}[label=\thesection.\arabic*]
\item
The command
\begin{lstlisting}
	output_signal = signal.lfilter(b, a, input_signal)
	\end{lstlisting}
in Problem \ref{prob:output} is executed through the following difference equation
\begin{equation}
\label{eq:iir_filter_gen}
 \sum _{m=0}^{M}a\brak{m}y\brak{n-m}=\sum _{k=0}^{N}b\brak{k}x\brak{n-k}
\end{equation}
%
where the input signal is $x(n)$ and the output signal is $y(n)$ with initial values all 0. Replace
\textbf{signal.filtfilt} with your own routine and verify.
%
\item Repeat all the exercises in the previous sections for the above $a$ and $b$.

\item What is the sampling frequency of the input signal?
\\
\solution
Sampling frequency(fs)=44.1kHZ.
\item
What is type, order and  cutoff-frequency of the above butterworth filter
\\
\solution
The given butterworth filter is low pass with order=2 and cutoff-frequency=4kHz.
%
\item
Modifying the code with different input parameters and to get the best possible output.
%
\end{enumerate}

\end{document}